Isabelle2/DMultiPaxosCorrectness.thy
@@ -1,0 +1,348 @@
+theory DMultiPaxosCorrectness
+imports "../../IO-Automata/Simulations" "../../IO-Automata/IOA_Automation" 
+  "~~/src/HOL/Library/Monad_Syntax" "~~/src/HOL/Library/Code_Target_Numeral"
+  "~~/src/HOL/Library/FinFun_Syntax"
+begin
+
+type_synonym acc = nat
+type_synonym bal = nat
+type_synonym inst = nat
+typedecl cmd
+consts accs :: "acc set"
+
+datatype msgs = 
+  Msg1a bal|
+  Msg1b acc inst bal "bal \<times> cmd option"|
+  Msg2a inst bal cmd
+
+record acc_state =
+  ballot :: "bal"
+  vote :: "inst \<Rightarrow>f bal \<Rightarrow>f cmd option"
+
+record mp_state = 
+  ballot :: "acc \<Rightarrow>f bal"
+  vote ::"acc \<Rightarrow>f inst \<Rightarrow>f bal \<Rightarrow>f cmd option"
+  network :: "msgs set"
+  propCmds :: "cmd option set"
+
+definition maxAcceptorVote::"acc \<Rightarrow> inst \<Rightarrow> mp_state \<Rightarrow> (bal \<times> cmd option)" where
+  "maxAcceptorVote a i s \<equiv> 
+    let bals = finfun_to_list ((vote s) $ a $ i);
+      bals_flt = (filter (\<lambda>b. (((vote s) $ a $ i) $ b) \<noteq> None) bals) @ [0];
+      maxBal = (fold max bals_flt (bals_flt!0));
+      v = (if maxBal > 0 then (((vote s) $ a $ i) $ maxBal) else None) in
+    (maxBal, v)"
+
+definition safe_at where
+  "safe_at m1bmsgs \<equiv> (let 
+    m1bnum = card m1bmsgs in
+    if (m1bnum * 2 > card accs) then True
+    else False)"
+
+definition safeVote::"msgs set \<Rightarrow> mp_state \<Rightarrow> cmd option set" where
+  "safeVote m1bmsgs state \<equiv> let 
+      m1bpair = image (\<lambda>nm. case nm of (Msg1b _ _ _ vs) \<Rightarrow> vs) m1bmsgs;
+      m1bBal = image (\<lambda>x. fst x) m1bpair;
+      maxBal = the_elem (Set.bind (Set.filter (\<lambda>le. \<forall>x \<in> m1bBal. x \<le> le) m1bBal) (\<lambda>x. {x}));
+      maxVal = image (\<lambda>x. snd x) (Set.filter (\<lambda>le. fst le = maxBal) m1bpair);
+      safeVal = Set.remove None maxVal in
+   if (safeVal \<noteq> {}) then safeVal else propCmds state"
+
+inductive_set reach :: "mp_state set"
+where
+init:
+  "\<lparr> ballot = (K$ 0), vote = (K$ K$ K$ None),
+    network = {}, propCmds = {}\<rparr> \<in> reach"
+| propose:
+  "\<lbrakk> s \<in> reach; c \<notin> propCmds s \<rbrakk> \<Longrightarrow>
+    s\<lparr> propCmds := (propCmds s) \<union> {c} \<rparr> \<in> reach"
+| phase1a:
+  "\<lbrakk> s \<in> reach; b > 0; Msg1a b \<notin> network s \<rbrakk> \<Longrightarrow>
+    s\<lparr> network := (network s) \<union> {Msg1a b} \<rparr> \<in> reach"
+| phase1b:
+  "\<lbrakk> s \<in> reach; Msg1a b \<in> network s; a \<in> accs; 
+    (ballot s) $ a < b; s1 = s\<lparr>ballot := (ballot s)(a $:= b)\<rparr>;
+    (maxBal, v) = (maxAcceptorVote a i s1); Msg1b a i b (maxBal, v) \<notin> network s \<rbrakk> \<Longrightarrow>
+    s1\<lparr> network := (network s) \<union> {Msg1b a i b (maxBal,v)} \<rparr> \<in> reach"
+| phase2a:
+  "\<lbrakk> s \<in> reach; 
+    m2anum = card (Set.filter (\<lambda>nm. case nm of Msg2a i2 b2 _ \<Rightarrow> (i2 = i \<and> b2 = b)| _ \<Rightarrow> False) (network s)); m2anum = 0; 
+    m1bmsgs = Set.filter (\<lambda>nm. case nm of Msg1b _ i2 b2 _ \<Rightarrow> (i2 = i \<and> b2 = b)| _ \<Rightarrow> False) (network s);
+    safe_at m1bmsgs; safeVal = safeVote m1bmsgs s; Some c \<in> safeVal \<rbrakk> \<Longrightarrow>
+    s\<lparr> network := (network s) \<union> {Msg2a i b c} \<rparr> \<in> reach"
+| vote_cmd:
+  "\<lbrakk> s \<in> reach; a \<in> accs; b = (ballot s) $ a; Msg2a i b c \<in> network s\<rbrakk> \<Longrightarrow>
+    s\<lparr> vote := (vote s)(a $:= ((vote s) $ a) (i $:= ((vote s) $ a $ i)(b $:= Some c))) \<rparr> \<in> reach"
+
+lemma set_joint[simp]:
+  assumes "finite accs" and "q1 \<subseteq> accs" and "q2 \<subseteq> accs" and 
+  "2 * card q1 > card accs" and "2 * card q2 > card accs"
+  shows "q1 \<inter> q2 \<noteq> {}"
+proof
+  assume "q1 \<inter> q2 = {}"
+  hence 1:"card q1 + card q2 \<le> card accs" using assms(1,2,3)
+    by (metis Un_subset_iff card_Un_disjoint card_mono finite_subset)
+  have 2:"card q1 + card q2 > card accs" using assms(4,5)
+    using add.commute add_less_imp_less_right le_less_trans less_imp_le_nat mult_2 not_le by linarith
+  thus "False" using "1" leD by blast
+qed
+
+lemma set_prop[simp]:
+  assumes "m2anum = card (Set.filter (\<lambda>nm. case nm of Msg2a i2 b2 x \<Rightarrow> i2 = i \<and> b2 = b
+    | _ \<Rightarrow> False) s)" and "m2anum = 0" and "finite s"
+  shows "Msg2a i b c \<notin> s"
+proof
+  assume "Msg2a i b c \<in> s"
+  hence "Msg2a i b c \<in> (Set.filter (\<lambda>nm. case nm of Msg2a i2 b2 x \<Rightarrow> i2 = i \<and> b2 = b | _ \<Rightarrow> False) s)" by simp
+  hence "(Set.filter (\<lambda>nm. case nm of Msg2a i2 b2 x \<Rightarrow> i2 = i \<and> b2 = b | _ \<Rightarrow> False) s) \<noteq> {}" by blast
+  hence "m2anum \<noteq> 0" using assms(1,3)
+    by (simp add: Collect_mem_eq Finite_Set.card_0_eq Set.filter_def finite_Collect_conjI)
+  thus "False" using assms(2) by blast
+qed
+
+lemma cmd_safe[simp]:
+  assumes "s \<in> reach" and "Msg2a i b c \<in> network s" and "finite accs" and "finite (network s)"
+  shows "2 * card (Set.filter (\<lambda>nm. case nm of Msg1b _ i2 b2 _ \<Rightarrow> (i2 = i \<and> b2 = b)| _ \<Rightarrow> False) (network s)) > card accs"
+using assms
+proof(induct set: reach)
+  case (init)
+    show ?case using init.prems(1) by auto 
+next
+  case (propose s v)
+    have " Msg2a i b c \<in> network s" using propose.prems(1)
+      by (simp add: mp_state.ext_inject mp_state.surjective mp_state.update_convs(4))
+    thus ?case using propose.prems(2,3) propose.hyps(2)
+      using mp_state.iffs mp_state.surjective mp_state.update_convs(4) by auto
+next
+  case (phase1a s)
+  have " Msg2a i b c \<in> network s" using phase1a.prems(1)
+    by (simp add: Un_empty_right Un_insert_right insertE mp_state.ext_inject mp_state.surjective mp_state.update_convs(3) msgs.simps(7))
+  thus ?case using phase1a.prems(2,3) phase1a.hyps(2)
+    by (smt Collect_cong Set.filter_def Un_insert_right finite_Un insert_iff mp_state.ext_inject mp_state.surjective mp_state.update_convs(3) msgs.simps(10) sup_bot.right_neutral)  
+next
+  case (vote_cmd s a' b' i' c')
+  have " Msg2a i b c \<in> network s" using vote_cmd.prems(1)
+    by (simp add: mp_state.ext_inject mp_state.surjective mp_state.update_convs(2))
+  thus ?case using vote_cmd.prems(2,3) vote_cmd.hyps(2)
+    by (simp add: mp_state.ext_inject mp_state.surjective mp_state.update_convs(2))
+next
+  case (phase1b s b' a' s1 maxB v' i')
+  have " Msg2a i b c \<in> network s" using phase1b.prems(1)
+    using UnE mp_state.ext_inject mp_state.surjective mp_state.update_convs(3) msgs.simps(9) singletonD by auto
+  hence 0:"card accs < 2 * card (Set.filter (\<lambda>a. case a of Msg1b x i2 b2 xa \<Rightarrow> i2 = i \<and> b2 = b | _ \<Rightarrow> False) (network s))"
+    using phase1b.prems(2,3) phase1b.hyps(2)
+      by (simp add: finite_Un mp_state.select_convs(3) mp_state.surjective mp_state.update_convs(3))
+  have "(network s) \<subseteq> (network (s1\<lparr>network := network s \<union> {Msg1b a' i' b' (maxB, v')}\<rparr>))"
+    by (simp add: Un_empty_right Un_insert_right mp_state.ext_inject mp_state.surjective mp_state.update_convs(3) subset_insertI)
+  hence 1:"Set.filter (\<lambda>a. case a of Msg1b x i2 b2 xa \<Rightarrow> i2 = i \<and> b2 = b | _ \<Rightarrow> False) (network s) \<subseteq>
+    Set.filter (\<lambda>a. case a of Msg1b x i2 b2 xa \<Rightarrow> i2 = i \<and> b2 = b | _ \<Rightarrow> False) (network (s1\<lparr>network := network s \<union> {Msg1b a' i' b' (maxB, v')}\<rparr>))"
+      by (simp add: subset_eq)
+  have "finite (Set.filter (\<lambda>a. case a of Msg1b x i2 b2 xa \<Rightarrow> i2 = i \<and> b2 = b | _ \<Rightarrow> False) (network (s1\<lparr>network := network s \<union> {Msg1b a' i' b' (maxB, v')}\<rparr>)))"
+    using phase1b.prems(3)
+      by (simp add: Collect_mem_eq Set.filter_def finite_Collect_conjI)
+  hence "card (Set.filter (\<lambda>a. case a of Msg1b x i2 b2 xa \<Rightarrow> i2 = i \<and> b2 = b | _ \<Rightarrow> False) (network s)) \<le>
+    card (Set.filter (\<lambda>a. case a of Msg1b x i2 b2 xa \<Rightarrow> i2 = i \<and> b2 = b | _ \<Rightarrow> False) (network (s1\<lparr>network := network s \<union> {Msg1b a' i' b' (maxB, v')}\<rparr>)))"
+      using phase1b.prems(3) 1 card_mono by blast 
+  thus ?case using 0 using le_less_trans nat_mult_less_cancel_disj not_le by linarith 
+next
+  case (phase2a s m2anum i' b' m1bmsgs safeVal c')
+  thus ?case
+  proof(cases "i = i' \<and> b = b'")
+    case True
+    hence 0:"card accs < 2 * card (Set.filter (\<lambda>nm. case nm of
+      Msg1b x i2 b2 xa \<Rightarrow> i2 = i \<and> b2 = b | _ \<Rightarrow> False) (network s))" using phase2a.hyps(5,6) unfolding safe_at_def
+        using mult.commute by presburger
+    have "(Set.filter (\<lambda>nm. case nm of Msg1b x i2 b2 xa \<Rightarrow> i2 = i \<and> b2 = b
+      | _ \<Rightarrow> False) (network s)) \<subseteq> (Set.filter (\<lambda>a. case a of  Msg1b x i2 b2 xa \<Rightarrow> i2 = i \<and> b2 = b
+        | _ \<Rightarrow> False) (network (s\<lparr>network :=  network s \<union> {Msg2a i' b' c'}\<rparr>)))" by auto
+    hence "card (Set.filter (\<lambda>nm. case nm of Msg1b x i2 b2 xa \<Rightarrow> i2 = i \<and> b2 = b
+      | _ \<Rightarrow> False) (network s)) \<le> card (Set.filter (\<lambda>a. case a of  Msg1b x i2 b2 xa \<Rightarrow> i2 = i \<and> b2 = b
+        | _ \<Rightarrow> False) (network (s\<lparr>network :=  network s \<union> {Msg2a i' b' c'}\<rparr>)))" using phase2a.prems(3)
+          by (simp add: Collect_mem_eq Set.filter_def card_mono finite_Collect_conjI)
+    thus ?thesis  using 0 le_less_trans nat_mult_less_cancel_disj not_le by linarith
+  next
+    case False
+    hence "Msg2a i b c \<in> network s" using phase2a.prems(1)
+      using Un_insert_right insert_iff mp_state.cases mp_state.select_convs(3) mp_state.update_convs(3) msgs.inject(3) sup_bot.right_neutral by auto
+    hence "card accs < 2 * card (Set.filter (\<lambda>a. case a of Msg1b x i2 b2 xa \<Rightarrow> i2 = i \<and> b2 = b
+      | _ \<Rightarrow> False) (network s))" using phase2a.prems(2,3) phase2a.hyps(2)
+        by (simp add: finite_Un mp_state.ext_inject mp_state.surjective mp_state.update_convs(3))
+    thus ?thesis
+      by (smt Collect_cong Set.filter_def Un_insert_right insert_iff mp_state.ext_inject mp_state.surjective mp_state.update_convs(3) msgs.simps(12) sup_bot.comm_neutral)
+  qed
+qed
+  
+lemma single_i_b[simp]:
+  assumes "s \<in> reach" and "Msg2a i b c \<in> network s" and "finite accs" and "finite (network s)"
+  shows "card (Set.filter (\<lambda>nm. case nm of Msg2a i2 b2 _ \<Rightarrow> (i2 = i \<and> b2 = b)| _ \<Rightarrow> False) (network s)) = 1"
+using assms
+proof(induct set: reach)
+  case init
+    thus ?case by (simp add: equals0D mp_state.select_convs(3))
+next
+  case propose
+    thus ?case using mp_state.iffs mp_state.surjective mp_state.update_convs(4) by fastforce
+next
+  case (phase1a s b')
+    have "Msg2a i b c \<in> network s" using phase1a.prems(1)
+      by (simp add: UnE empty_iff insert_iff mp_state.select_convs(3) mp_state.surjective mp_state.update_convs(3) msgs.distinct(3)) 
+    thus ?case using phase1a.prems(2,3) phase1a.hyps(2)
+      by (smt Collect_cong Set.filter_def Un_insert_right finite_Un insert_iff mp_state.ext_inject mp_state.surjective mp_state.update_convs(3) msgs.simps(10) sup_bot.right_neutral)
+next
+  case (vote_cmd s a' b' i' c')
+  have " Msg2a i b c \<in> network s" using vote_cmd.prems(1)
+    by (simp add: mp_state.ext_inject mp_state.surjective mp_state.update_convs(2))
+  thus ?case using vote_cmd.prems(2,3) vote_cmd.hyps(2)
+    using mp_state.ext_inject mp_state.surjective mp_state.update_convs(2) by fastforce  
+next
+  case (phase1b s b' a' s1 maxBal v' i')
+    have 0:"Msg2a i b c \<in> network s" using phase1b.prems(1)
+      by (simp add: Un_insert_right insert_iff mp_state.cases mp_state.select_convs(3) mp_state.update_convs(3) msgs.simps(9) sup_bot.right_neutral)
+    have "finite (network s)" using phase1b.prems(3)
+      by (simp add: finite_Un mp_state.select_convs(3) mp_state.surjective mp_state.update_convs(3))
+    hence 1:"card (Set.filter(\<lambda>a. case a of  Msg2a i2 b2 x \<Rightarrow> i2 = i \<and> b2 = b | _ \<Rightarrow> False) (network s)) = 1" 
+      using 0 phase1b.prems(2) phase1b.hyps(2) by blast
+    hence "card (Set.filter(\<lambda>a. case a of  Msg2a i2 b2 x \<Rightarrow> i2 = i \<and> b2 = b | _ \<Rightarrow> False) (network s1)) = 1" 
+      using phase1b.hyps(6) by (simp add: mp_state.ext_inject mp_state.surjective mp_state.update_convs(1))
+    thus ?case using 1
+      by (smt Collect_cong Set.filter_def UnCI Un_insert_right insertE mp_state.select_convs(3) mp_state.surjective mp_state.update_convs(3) msgs.case(2) sup_bot.comm_neutral) 
+next
+  case (phase2a s m2anum i' b' m1bmsgs safeVal c')
+    thus ?case
+    proof(cases "i = i' \<and> b = b'")
+      case True
+        assume 0:"i = i' \<and> b = b'"
+        hence "card (Set.filter (\<lambda>a. case a of Msg2a i2 b2 x \<Rightarrow> i2 = i \<and> b2 = b
+          | _ \<Rightarrow> False) (network s)) = 0" using phase2a.hyps(3,4) by auto
+        hence "Set.filter (\<lambda>a. case a of Msg2a i2 b2 x \<Rightarrow> i2 = i \<and> b2 = b
+          | _ \<Rightarrow> False) (network s) = {}" using phase2a.prems(3)
+            by (simp add: Collect_mem_eq Set.filter_def card_0_eq finite_Collect_conjI finite_Un mp_state.select_convs(3) mp_state.surjective mp_state.update_convs(3))
+        hence "Set.filter (\<lambda>a. case a of Msg2a i2 b2 x \<Rightarrow> i2 = i \<and> b2 = b
+          | _ \<Rightarrow> False) (network(s\<lparr>network :=  network s \<union> {Msg2a i' b' c'}\<rparr>)) = {Msg2a i b c'}" using 0
+            using CollectD Collect_cong Set.filter_def Un_iff insertI2 member_filter mp_state.ext_inject mp_state.surjective mp_state.update_convs(3) msgs.simps(12) singletonI singleton_conv2 by auto    
+        thus ?thesis using phase2a.prems(3) by auto
+    next
+      case False
+        assume 1:"\<not> (i = i' \<and> b = b')"
+        hence "Msg2a i b c \<in> network s" using phase2a.prems(1,3) by auto
+        hence "card (Set.filter (\<lambda>a. case a of Msg2a i2 b2 x \<Rightarrow> i2 = i \<and> b2 = b | _ \<Rightarrow> False) (network s)) = 1"
+          using phase2a.hyps(2) phase2a.prems(2,3) finite_Un mp_state.ext_inject mp_state.surjective mp_state.update_convs(3) by fastforce
+        thus ?thesis using 1
+          by (smt Collect_cong Set.filter_def Un_insert_right insert_iff mp_state.ext_inject mp_state.surjective mp_state.update_convs(3) msgs.simps(12) sup_bot.comm_neutral)
+    qed
+qed
+
+lemma single_i_b_c[simp]:
+  assumes "s \<in> reach" and "Msg2a i b c \<in> network s" and "finite accs" and "finite (network s)"
+  shows "Set.filter (\<lambda>nm. case nm of Msg2a i2 b2 _ \<Rightarrow> (i2 = i \<and> b2 = b)| _ \<Rightarrow> False) (network s) = {Msg2a i b c}"
+proof-
+  have "card (Set.filter (\<lambda>nm. case nm of  Msg2a i2 b2 x \<Rightarrow> i2 = i \<and> b2 = b
+    | _ \<Rightarrow> False) (network s)) = 1" using assms single_i_b by blast
+  thus ?thesis using assms(2,4)
+    by (smt Collect_cong Set.filter_def card_eq_1_iff mem_Collect_eq msgs.simps(12) singleton_conv2)
+qed
+
+lemma vote_msg2a[simp]:
+  assumes "s \<in> reach" and "(vote s) $ a $ i $ b = Some c" and "finite accs" and "finite (network s)"
+  shows "Msg2a i b c \<in> network s"
+using assms
+proof(induct set: reach)
+  case init
+    thus ?case by (simp add: finfun_const_apply mp_state.select_convs(2) option.distinct(1))
+next
+  case propose
+    thus ?case by (metis mp_state.ext_inject mp_state.surjective mp_state.update_convs(4))
+next
+  case phase1a
+    thus ?case by (metis UnCI finite_Un mp_state.ext_inject mp_state.surjective mp_state.update_convs(3)) 
+next
+  case phase1b
+    thus ?case
+      by (metis UnCI finite_Un mp_state.ext_inject mp_state.surjective mp_state.update_convs(1) mp_state.update_convs(3)) 
+next
+  case phase2a
+    thus ?case by (metis UnCI finite_Un mp_state.ext_inject mp_state.surjective mp_state.update_convs(3))
+next
+  case vote_cmd
+    thus ?case
+      by (smt finfun_upd_apply_same finfun_upd_triv finfun_update_twist mp_state.ext_inject mp_state.surjective mp_state.update_convs(2) mp_state.update_convs(5) option.inject) 
+qed
+
+lemma safe_inv[simp]:
+  assumes "s \<in> reach" and "finite accs" and "finite (network s)" and "acc\<^sub>1 \<in> accs" and "acc\<^sub>2 \<in> accs" and "acc\<^sub>1 \<noteq> acc\<^sub>2"
+  and "cmd1 = ((vote s) $ acc\<^sub>1 $ i $ b)" and "cmd2 = ((vote s) $ acc\<^sub>2 $ i $ b)" and "cmd1 \<noteq> None" and "cmd2 \<noteq> None"
+  shows "cmd1 = cmd2"
+using assms
+proof(induct set: reach)
+  case init
+    thus ?case by (simp add: finfun_const_apply mp_state.select_convs(2))
+next
+  case (propose s v)
+    thus ?case by (simp add: mp_state.ext_inject mp_state.surjective mp_state.update_convs(4))
+next
+  case phase1a
+    thus ?case by (simp add: mp_state.ext_inject mp_state.surjective mp_state.update_convs(3))
+next
+  case phase2a
+    thus ?case by (metis finite_Un mp_state.ext_inject mp_state.surjective mp_state.update_convs(3)) 
+next
+  case (phase1b s b' a' s1 maxNal v' i')
+    thus ?case
+      by (simp add: mp_state.ext_inject mp_state.surjective mp_state.update_convs(1) mp_state.update_convs(3)) 
+next
+  case (vote_cmd s a' b' i' c')
+    print_cases
+    thus ?case
+    proof(cases "acc\<^sub>1 = a' \<and> i = i' \<and> b = b'")
+      case True
+        print_cases
+        assume 0:"acc\<^sub>1 = a' \<and> i = i' \<and> b = b'"
+        have 1:"i = i' \<and> b = b'" using 0 by blast
+        have 2:"cmd2 = (vote s) $ acc\<^sub>2 $ i $ b" using vote_cmd.prems(7,5) 0
+          by (simp add: finfun_upd_apply mp_state.ext_inject mp_state.surjective mp_state.update_convs(2))
+        have 3:"cmd1 = Some c'" using vote_cmd.prems(6) 0
+          by (simp add: finfun_upd_apply mp_state.ext_inject mp_state.surjective mp_state.update_convs(2))
+        hence "Msg2a i b c' \<in> network (s\<lparr>vote := (vote s)(a' $:= (vote s $ a')(i' $:= (vote s $ a' $  i')(b' $:= Some
+          c')))\<rparr>)" using vote_cmd.prems(6) 1 vote_cmd.hyps(5) vote_msg2a
+            by (metis (no_types, lifting) mp_state.ext_inject mp_state.surjective mp_state.update_convs(2) mp_state.update_convs(5)) 
+        hence 4:"Msg2a i b c' \<in> network s" using 1 vote_cmd.hyps(5) by blast
+        have "Msg2a i b (the cmd2) \<in> network s" using 2 vote_cmd.hyps(1) vote_cmd.prems(1,2,9) vote_msg2a
+          by (metis (no_types, lifting) mp_state.ext_inject mp_state.surjective mp_state.update_convs(2) mp_state.update_convs(5) option.exhaust_sel) 
+        hence "Some c' = cmd2" using 3 4 assms(1,2,3,7,8) single_i_b_c
+          by (metis msgs.inject(3) option.collapse the_elem_eq vote_cmd.prems(9) vote_msg2a)
+        thus ?thesis using 3 by auto
+    next
+      case False
+        assume 0:"\<not>(acc\<^sub>1 = a' \<and> i = i' \<and> b = b')"
+        thus ?thesis
+        proof(cases "acc\<^sub>2 = a' \<and> i = i' \<and> b = b'")
+          case True
+            assume 1:"acc\<^sub>2 = a' \<and> i = i' \<and> b = b'"
+            hence 2:"i = i' \<and> b = b'" by blast
+            have 3:"cmd1 = (vote s) $ acc\<^sub>1 $ i $ b" using vote_cmd.prems(6,5) 1
+              by (simp add: finfun_upd_apply mp_state.ext_inject mp_state.surjective mp_state.update_convs(2))
+            have 4:"cmd2 = Some c'" using vote_cmd.prems(7) 1
+              by (simp add: finfun_upd_apply mp_state.ext_inject mp_state.surjective mp_state.update_convs(2))
+            hence "Msg2a i b c' \<in> network (s\<lparr>vote := (vote s)(a' $:= (vote s $ a')(i' $:= (vote s $ a' $  i')(b' $:= Some
+              c')))\<rparr>)" using vote_cmd.prems(7) 2 vote_cmd.hyps(5) vote_msg2a
+                by (metis (no_types, lifting) mp_state.ext_inject mp_state.surjective mp_state.update_convs(2) mp_state.update_convs(5)) 
+            hence 5:"Msg2a i b c' \<in> network s" using 2 vote_cmd.hyps(5) by blast
+            have "Msg2a i b (the cmd1) \<in> network s" using 3 assms(2,3) vote_cmd.hyps(1) vote_cmd.prems(1,2,8) vote_msg2a
+              by (metis (no_types, lifting) mp_state.ext_inject mp_state.surjective mp_state.update_convs(2) mp_state.update_convs(5) option.exhaust_sel) 
+            hence "Some c' = cmd1" using 4 5 vote_cmd.prems(1,8) assms(1,3,7,8) vote_msg2a single_i_b_c
+              by (metis msgs.inject(3) option.collapse the_elem_eq)
+            thus ?thesis using 4 by auto
+        next
+          case False
+            assume 1:"\<not>(acc\<^sub>2 = a' \<and> i = i' \<and> b = b')"
+            have 2:"cmd1 = (vote s) $ acc\<^sub>1 $ i $ b" using vote_cmd.prems(6) 0
+              by (smt finfun_upd_apply_same finfun_upd_triv finfun_update_twist mp_state.ext_inject mp_state.surjective mp_state.update_convs(2) mp_state.update_convs(5))
+            have "cmd2 = (vote s) $ acc\<^sub>2 $ i $ b" using vote_cmd.prems(7) 1
+              by (smt finfun_upd_apply_same finfun_upd_triv finfun_update_twist mp_state.ext_inject mp_state.surjective mp_state.update_convs(2) mp_state.update_convs(5))
+            thus ?thesis using 2 vote_cmd.prems(1,2,3,4,5,8,9) vote_cmd.hyps(2)
+              by (simp add: mp_state.ext_inject mp_state.surjective mp_state.update_convs(2))
+        qed
+  qed
+qed
+
+end
